\documentclass[12pt,english]{article}
\usepackage[a4paper,bindingoffset=0.2in,%
left=1in,right=1in,top=1in,bottom=1in,%
footskip=.25in]{geometry}
\usepackage{amsmath}
\usepackage{amssymb}
\begin{document}
	\section{Energy}
	\begin{equation}
	\begin{split}
		U_{tot}  = &\sum_{i=1}^{N} [E_i^0 + \chi_i q_i + \tilde{\chi_i}\tilde{q_i }+ \frac{1}{2}(J_{ii}+\frac{2\gamma_{ii}}{\sqrt{\pi}})q_i^2 + \frac{1}{2}(\tilde{J_{ii}}+\frac{2\tilde{\gamma_{ii}}}{\sqrt{\pi}})\tilde{q_i}^2+\frac{q_i\tilde{q_i }(\gamma_{ii}'+\gamma_{ii}'')}{\sqrt{\pi}}]\\ 
		&+\sum_{i>j} q_iq_j\frac{erf(\gamma_{ij}r_{ij})}{r_{ij}} + \sum_{i>j} q_i\tilde{q_j}\frac{erf(\gamma_{ij}'r_{ij})}{r_{ij}}\\
		 &+\sum_{i>j}\tilde{q_i }q_j \frac{erf(\gamma_{ij}''r_{ij})}{r_{ij}} + \sum_{i>j}\tilde{q_i}\tilde{q_j} \frac{erf(\tilde{\gamma_{ij}}r_{ij})}{r_{ij}}
	\end{split}
	\end{equation}
	\newline
	\begin{equation}
		\begin{split}
			&\frac{\partial U_{tot}}{\partial q_i}=0 ; \forall i = 1 ,...,N \\
			& = \chi_i 
			+ (J_{ii}+\frac{2\gamma_{ii}}{\sqrt{\pi}})q_i 
			+ \frac{(\gamma_{ii}'+ \gamma_{ii}'')}{\sqrt{\pi}}\tilde{q_i} 
			+ \frac{erf(\gamma_{ij}r_{ij})}{r_{ij}}q_j 
			+ \frac{erf(\gamma_{ij}'r_{ij})}{r_{ij}}\tilde{q_j}
		\end{split}
	\end{equation}
	\begin{equation}
		\begin{split}
			&\frac{\partial U_{tot}}{\partial \tilde{q_i}}=0 ; \forall i = 1 ,..., N  \\
			& = \tilde{\chi_i} 
			+ (\tilde{J_{ii}} + \frac{2\tilde{\gamma_{ii}}}{\sqrt{\pi}})\tilde{q_i } 
			+ \frac{(\gamma_{ii}' + \gamma_{ii}'')}{\sqrt{\pi}}q_i 
			+ \frac{erf(\gamma_{ij}''r_{ij})}{r_{ij}}q_j 
			+ \frac{erf(\tilde{q_j}r_{ij})}{r_{ij}}\tilde{q_j}
		\end{split}		
	\end{equation}
	\begin{equation}
	\begin{split}
			\gamma_{ij} = \frac{1}{\sqrt{\alpha_i^2+\alpha_j^2}}
			\hspace{0.25\textwidth} 
			\gamma_{ij}'=\frac{1}{\sqrt{\alpha_i^2+\tilde{\alpha_j}^2}}\\	
			\gamma_{ij}''=\frac{1}{\sqrt{\tilde{\alpha_i}^2+\alpha_j^2}}
			\hspace{0.25\textwidth} 
			\tilde{\gamma_{ij}} = \frac{1}{\sqrt{\tilde{\alpha_i}^2+\tilde{\alpha_j}^2}}
	\end{split}
	\end{equation}
	\newline
	\begin{equation}
		A_{ij}=\frac{\partial U_{tot}}{\partial q_i \partial q_j} = 
		\begin{cases}
			J_{ii}+\frac{2\gamma_{ii}}{\sqrt{\pi}} & i =j\\
			\frac{erf(\gamma_{ij}r_{ij})}{r_{ij}} & i \neq j
		\end{cases}
	\end{equation}
	\begin{equation}
		C_{ij}=\frac{\partial U_{tot}}{\partial q_i \partial \tilde{q_j}} =
		\begin{cases}
			\frac{\gamma_{ii}'+\gamma_{ii}''}{\sqrt{\pi}} & i=j \\
			\frac{erf(\gamma_{ij}'r_{ij})}{r_{ij}} & i\neq j
		\end{cases}
	\end{equation}
	\begin{equation}
		B_{ij}=\frac{\partial U_{tot}}{\partial \tilde{q_i} \partial \tilde{q_j}} =
		\begin{cases}
			\tilde{J_{ii}}+\frac{2\tilde{\gamma_{ii}}}{\sqrt{\pi}} & i=j\\
			\frac{erf(\tilde{\gamma_{ij}}r_{ij})}{r_{ij}} & i \neq j
		\end{cases}
	\end{equation}
	\begin{equation}
		D_{ij}=\frac{\partial U_{tot}}{\partial \tilde{q_i} \partial q_j} = 
		\begin{cases}
			\frac{\gamma_{ii}'+\gamma_{ii}''}{\sqrt{\pi}} & i=j \\
			\frac{erf(\gamma_{ij}''r_{ij})}{r_{ij}} & i\neq j
		\end{cases}
	\end{equation}
	\begin{equation}
		\Lambda Q = \Xi \hspace{10pt} ; \hspace{10pt}  \Lambda =
	\begin{pmatrix}
		A & C \\
		D & B
	\end{pmatrix}
	\end{equation}	
	\begin{equation}
		\begin{split}
			q+\tilde{q} = &[-(B-DA^{-1}C)^{-1}+(A-CB^{-1}D)^{-1}CB^{-1}]\tilde{\chi} \\
						  &[(B-DA^{-1}C)^{-1}DA^{-1} - (A-CB^{-1}D)^{-1}]\chi 
		\end{split}
	\end{equation}
	\rule{450pt}{0.5pt}
	\section{CEP}
	\begin{equation}
	A Q = \Xi\hspace{10pt} ; 
	A = 
	\begin{pmatrix}
		A & C & \vline & 1\\
		D & B & \vline & 1\\
		\hline
		1 & 1 & \vline & 0
	\end{pmatrix}
	\hspace{10pt}
	Q = 
	\begin{pmatrix}
		q_1 \\ q_2 \\ .\\.\\.\\q_n\\\tilde{q_1}\\\tilde{q_2}\\.\\.\\.\\\tilde{q_n}\\\hline\lambda
	\end{pmatrix}
	\hspace{10pt}
	\Xi = 
	\begin{pmatrix}
	-\chi_1 \\ -\chi_2 \\ .\\.\\.\\-\chi_n\\-\tilde{\chi_1}\\-\tilde{\chi_2}\\.\\.\\.\\-\tilde{\chi_n}\\\hline q_{tot}
	\end{pmatrix}
	\end{equation}
	\begin{equation}
		\implies
		Q = A^{-1}\Xi
	\end{equation}
	
\end{document}
